AP/Game/Basic.lean
@@ -1,19 +1,21 @@
 import AP.Game.Defs
 
+open Util.Data
+
 namespace Game
 
 universe u
 variable {T : GameParams.{u}} {game : Game T}
 
 theorem tr_eq_some_iff {a b} {t : T.Trans} :
-game.sys.tr a t = some b ↔ a.player = t.1 ∧ ∃ r,
-game.rules t.1 a.state t.2 = some r ∧ b =
-{ player := r.1
-, state := r.2
+game.sys.tr a t = some b ↔ a.player = t.1 ∧ ∃ p s',
+game.rules t.1 a.state t.2 = some ⟨p, s'⟩ ∧ p ∈ a.hist ∧ b =
+{ player := p
+, state := s'
 , hist := game.updateHist a t
 } := by
   simp only [game.h_sys_tr, GameParams.sys_tr, GameParams.updateHist,
-    Option.bind_eq_bind, Option.bind, Option.dite_none_right_eq_some,
+    ite_not, Option.bind_eq_bind, Option.bind, Option.dite_none_right_eq_some,
     updateHist, Prod.exists]
   constructor
   · rintro ⟨h₁, h₂⟩
@@ -22,25 +24,22 @@ game.rules t.1 a.state t.2 = some r ∧ b =
     nm x y z h₃
     use z.1, z.2
     simp [h₁, h₂, h₃]
-  · rintro ⟨h₁, x, y, h₂, rfl⟩
+  · rintro ⟨h₁, p, s', h₂, h₃, rfl⟩
     use h₁
-    simp [h₁, h₂]
+    simp [h₁, h₂, h₃]
 
 theorem trTo_iff {a b} {t : T.Trans} :
-game.sys.trTo a t b ↔ a.player = t.1 ∧ ∃ r,
-game.rules t.1 a.state t.2 = some r ∧ b =
-{ player := r.1
-, state := r.2
+game.sys.trTo a t b ↔ a.player = t.1 ∧ ∃ p s',
+game.rules t.1 a.state t.2 = some ⟨p, s'⟩ ∧ p ∈ a.hist ∧ b =
+{ player := p
+, state := s'
 , hist := game.updateHist a t
 } := tr_eq_some_iff
 
 @[simp]
-theorem player_mem_hist_initState {p' p s} : p' ∈ (T.initState p s).hist := by
+theorem mem_hist_initState {ps p s p'} :
+p' ∈ (T.initState ps p s).hist ↔ p' ∈ ps := by
   simp [GameParams.initState]
-
-theorem player_mem_hist_of_initial {p s} [h : game.sys.Initial s] : p ∈ s.hist := by
-  obtain ⟨p', s', rfl⟩ := game.h_sys_init_valid s
-  simp
 
 @[simp]
 theorem player_mem_updateHist_iff {p s t} :
@@ -50,32 +49,42 @@ p ∈ game.updateHist s t ↔ p ∈ s.hist := by
   · simp
   rfl
 
-theorem player_mem_hist_of_valid {a} [hv : game.sys.Valid a] {p} : p ∈ a.hist := by
+theorem mem_hist_iff_of_reachable {a b p} (hv : game.sys.Reachable a b) :
+p ∈ b.hist ↔ p ∈ a.hist := by
   classical
-  cases hv
-  nm s hs h
-  rw [System.reachable_iff_exi_trs] at h
-  obtain ⟨ts, h₁⟩ := h
-  induction ts using List.reverseRecOn generalizing a
-  · simp at h₁
-    subst h₁
-    exact game.player_mem_hist_of_initial
+  replace hv := System.exi_trs_of_reachable hv
+  obtain ⟨ts, h⟩ := hv
+  induction ts using List.reverseRecOn generalizing b
+  · simp at h
+    rw [h]
   nm ts t ih
-  simp [System.trs_append] at h₁
-  iterate split at h₁ <;> simp at h₁
-  nm h₂ x s' h₃; clear x
-  rcases h₁ with ⟨rfl, h₁⟩; clear h₁
-  generalize hb : game.sys.trs s ts = b at h₂ h₃
-  specialize @ih b.1 _
-  · simp [Prod.eq_iff_fst_eq_snd_eq, hb, h₂]
-  generalize b.1 = c at h₃ ih
-  clear! b
-  rw [tr_eq_some_iff] at h₃
-  obtain ⟨h₁, r, h₂, h₃, rfl⟩ := h₃
-  simpa
+  simp [System.trs_append] at h
+  iterate split at h
+  all_goals simp at h
+  nm h₁ x d h₂
+  rcases h with ⟨rfl, h⟩
+  clear h₁
+  generalize hr : game.sys.trs a ts = r at h h₂
+  rcases r with ⟨c, r⟩
+  subst h
+  dsimp at h₂
+  specialize ih hr
+  simp only [←ih]; clear ih
+  rw [tr_eq_some_iff] at h₂
+  obtain ⟨h₂, p, s', h₃, h₄, rfl⟩ := h₂
+  simp
+
+theorem mem_hist_of_reachable {a b p} (hv : game.sys.Reachable a b)
+(h : p ∈ a.hist) : p ∈ b.hist := by
+  rwa [game.mem_hist_iff_of_reachable hv]
+
+theorem mem_hist_of_reachable' {a b p} (hv : game.sys.Reachable a b)
+(h : p ∈ b.hist) : p ∈ a.hist := by
+  rw [game.mem_hist_iff_of_reachable hv] at h; exact h
 
 theorem hist_suffix_of_reachable {a} [hv : game.sys.Valid a] {b p}
-(h : game.sys.Reachable a b) : a.hist.get! p <:+ b.hist.get! p := by
+(h : game.sys.Reachable a b) (hp : p ∈ b.hist) :
+a.hist.get! p <:+ b.hist.get! p := by
   revert hv
   induction h using System.reachable_ind_right
   · intro hv
@@ -83,15 +92,26 @@ theorem hist_suffix_of_reachable {a} [hv : game.sys.Valid a] {b p}
   clear a b
   nm a b c t h₁ h₂ ih
   intro hv
-  specialize @ih _
+  have hb₁ : p ∈ b.hist :=
+    by
+      replace h₂ := System.reachable_of_tr h₂
+      exact mem_hist_of_reachable' h₂ hp
+  specialize @ih hb₁
   rw [tr_eq_some_iff] at h₂
-  rcases h₂ with ⟨h₂, ⟨p', c⟩, h₃, rfl⟩
+  rcases h₂ with ⟨h₂, p', c, h₃, h₄, rfl⟩
   simp [Game.updateHist, GameParams.updateHist, h₂]
   have hb := System.valid_of_reachable h₁
   rw [DMap.get!_map_eq_of_pos]
-  rotate_left
-  · exact game.player_mem_hist_of_valid
+  rotate_left; exact hb₁
   exact List.suffix_cons_of_suffix ih
+
+theorem exi_mem_hist_of_valid {a} [ha : game.sys.Valid a] : ∃ p, p ∈ a.hist := by
+  rw [System.valid_iff] at ha
+  obtain ⟨z, h₁, h₂⟩ := ha
+  obtain ⟨ps, p, s', rfl, h₄⟩ := game.h_sys_init_valid z
+  simp [GameParams.initState] at h₄
+
+#check 0 #exit
 
 theorem acyclic_gstate {a} [ha : game.sys.Valid a] : game.sys.Acyclic a := by
   rw [System.acyclic_iff]
@@ -105,11 +125,11 @@ theorem acyclic_gstate {a} [ha : game.sys.Valid a] : game.sys.Acyclic a := by
   replace h₁ := hist_suffix_of_reachable (p := p) h₁
   replace h₃ := hist_suffix_of_reachable (p := p) h₃
   rw [tr_eq_some_iff] at h₂
-  obtain ⟨h₂, ⟨p', t'⟩, h₄, rfl⟩:= h₂
+  obtain ⟨h₂, p', t', h₄, h₅, rfl⟩:= h₂
   simp at h₃
   clear! p'
   simp [updateHist, h₂, GameParams.updateHist] at h₃
-  rw [DMap.get!_map_eq_of_pos game.player_mem_hist_of_valid] at h₃
+  rw [DMap.get!_map_eq_of_pos] at h₃
   simp at h₃
 
 theorem validTr_iff {a} {t : T.Trans} :
