AP/Util/Main.lean
@@ -1,3 +1,3 @@
 import AP.Util.Basic
--- import AP.Util.Data.Set.Main
+import AP.Util.Data.Set.Main
 import AP.Util.Data.Map.Main
